src/named/SimpleSubst.v
@@ -1,0 +1,300 @@
+Require Import mathcomp.ssreflect.all_ssreflect.
+Set Implicit Arguments.
+Unset Strict Implicit.
+Unset Printing Implicit Defensive.
+Set Bullet Behavior "Strict Subproofs".
+
+
+From Ltac2 Require Import Ltac2.
+From Utils Require Import Utils.
+From Named Require Import Exp ARule ImCore Pf Interactive.
+Import Exp.Notations ARule.Notations.
+Require Import String.
+
+
+Require Coq.derive.Derive.
+
+Set Default Proof Mode "Ltac2".
+
+Set Default Proof Mode "Classic".
+
+
+Definition subst_lang : lang :=
+   [::[:> "G" : #"env", "A" : #"ty"
+       ----------------------------------------------- ("snoc_wkn_hd")
+       #"id" = #"snoc" #"wkn" #"hd" : #"sub" (#"ext" %"G" %"A") (#"ext" %"G" %"A")
+   ];
+   [:> "G1" : #"env", "G2" : #"env", "G3" : #"env",
+       "f" : #"sub" %"G1" %"G2",
+       "g" : #"sub" %"G2" %"G3",
+       "A" : #"ty",
+       "e" : #"el" %"G2" %"A"
+       ----------------------------------------------- ("cmp_snoc")
+       #"cmp" %"f" (#"snoc" %"g" %"e")
+       = #"snoc" (#"cmp" %"f" %"g") (#"el_subst" %"f" %"e")
+       : #"sub" %"G1" (#"ext" %"G3" %"A")
+   ];
+   [:> "G" : #"env", "G'" : #"env",
+       "g" : #"sub" %"G" %"G'",
+       "A" : #"ty",
+       "e" : #"el" %"G" %"A"
+       ----------------------------------------------- ("snoc_hd")
+       #"el_subst" (#"snoc" %"g" %"e") #"hd" = %"e"
+       : #"el" %"G" %"A"
+  ];
+  [:> "G" : #"env", "G'" : #"env",
+      "g" : #"sub" %"G" %"G'",
+      "A" : #"ty",
+      "e" : #"el" %"G" %"A"
+      ----------------------------------------------- ("wkn_snoc")
+      #"cmp" (#"snoc" %"g" %"e") #"wkn" = %"g" : #"sub" %"G" %"G'"
+  ];
+  [:| "G" : #"env", "A" : #"ty"
+       -----------------------------------------------
+       #"hd" : #"el" (#"ext" %"G" %"A") %"A"
+  ];
+  [:| "G" : #"env", "A" : #"ty"
+       -----------------------------------------------
+       #"wkn" : #"sub" (#"ext" %"G" %"A") %"G"
+  ];
+  [:| "G" : #"env", "G'" : #"env", "A" : #"ty",
+      "g" : #"sub" %"G" %"G'",
+      "e" : #"el" %"G" %"A"
+       -----------------------------------------------
+       #"snoc" "g" "e" : #"sub" %"G" (#"ext" %"G'" %"A")
+  ];
+  [:| "G" : #"env", "A": #"ty"
+       -----------------------------------------------
+       #"ext" "G" "A" : #"env"
+  ];
+  [:> 
+      ----------------------------------------------- ("id_emp_forget")
+      #"id" = #"forget" : #"sub" #"emp" #"emp"
+  ];
+  [:> "G" : #"env", "G'" : #"env", "g" : #"sub" %"G" %"G'"
+       ----------------------------------------------- ("cmp_forget")
+       #"cmp" %"g" #"forget" = #"forget" : #"sub" %"G" #"emp"
+  ];
+  [:| "G" : #"env" 
+      -----------------------------------------------
+      #"forget" : #"sub" %"G" #"emp"
+  ];
+  [:| 
+      -----------------------------------------------
+      #"emp" : #"env"
+  ];
+  [:> "G1" : #"env", "G2" : #"env", "G3" : #"env",
+       "f" : #"sub" %"G1" %"G2", "g" : #"sub" %"G2" %"G3",
+       "A" : #"ty", "e" : #"el" %"G3" %"A"
+       ----------------------------------------------- ("el_subst_cmp")
+       #"el_subst" %"f" (#"el_subst" %"g" %"e")
+       = #"el_subst" (#"cmp" %"f" %"g") %"e"
+       : #"el" %"G1" %"A"
+  ]; 
+  [:> "G" : #"env", "A" : #"ty", "e" : #"el" %"G" %"A"
+       ----------------------------------------------- ("el_subst_id")
+       #"el_subst" #"id" %"e" = %"e" : #"el" %"G" %"A"
+  ]; 
+  [:| "G" : #"env", "G'" : #"env", "g" : #"sub" %"G" %"G'",
+       "A" : #"ty", "e" : #"el" %"G'" %"A"
+       -----------------------------------------------
+       #"el_subst" "g" "e" : #"el" %"G" %"A"
+  ];
+  [s| "G" : #"env", "A" : #"ty"
+      -----------------------------------------------
+      #"el" "G" "A" srt
+  ];
+  [s|  
+      -----------------------------------------------
+      #"ty" srt
+  ];
+   [:> "G1" : #"env",
+         "G2" : #"env",
+         "G3" : #"env",
+         "G4" : #"env",
+         "f" : #"sub" %"G1" %"G2",
+         "g" : #"sub" %"G2" %"G3",
+         "h" : #"sub"%"G3" %"G4"
+         ----------------------------------------------- ("cmp_assoc")
+         #"cmp" %"f" (#"cmp" %"g" %"h") = #"cmp" (#"cmp" %"f" %"g") %"h" : #"sub" %"G1" %"G4"
+  ];  
+  [:> "G" : #"env", "G'" : #"env", "f" : #"sub" %"G" %"G'"
+       ----------------------------------------------- ("id_left")
+       #"cmp" #"id" %"f" = %"f" : #"sub" %"G"%"G'"
+  ];
+  [:> "G" : #"env", "G'" : #"env", "f" : #"sub" %"G" %"G'"
+      ----------------------------------------------- ("id_right")
+      #"cmp" %"f" #"id" = %"f" : #"sub" %"G" %"G'"
+  ];
+  [:| "G1" : #"env", "G2" : #"env", "G3" : #"env",
+       "f" : #"sub" %"G1" %"G2",
+       "g" : #"sub" %"G2" %"G3"
+       -----------------------------------------------
+       #"cmp" "f" "g" : #"sub" %"G1" %"G3"
+  ];
+  [:| "G" : #"env" 
+       -----------------------------------------------
+       #"id" : #"sub" %"G" %"G"
+  ];
+  [s| "G" : #"env", "G'" : #"env" 
+      -----------------------------------------------
+      #"sub" "G" "G'" srt                     
+  ];
+  [s|
+      -----------------------------------------------
+      #"env" srt
+   ]]%arule.
+
+
+(*
+invariants:
+
+ty := A
+env := . | env, ty | G
+...
+
+ *)
+
+Import OptionMonad.
+Definition simple_subst_to_pf_ty (e:exp) : option pf :=
+  match e with
+  | var x => Some (pvar x)
+  | _ => None
+  end.
+
+
+Fixpoint simple_subst_to_pf_env (e:exp) : option pf :=
+  match e with
+  | var x => Some (pvar x)
+  | con "emp" [::] => Some (pcon "emp" [::])
+  | con "ext" [:: A; G] =>
+    do pa <- simple_subst_to_pf_ty A;
+       pG <- simple_subst_to_pf_env G;
+       ret (pcon "ext" [:: pa; pG])
+  | _ => None
+  end.
+
+Definition simple_subst_to_pf_sort (t:sort) : option pf :=
+  match t with
+  | scon "env" [::] => Some (pcon "env" [::])
+  | scon "ty" [::] => Some (pcon "ty" [::])
+  | scon "sub" [:: G'; G] =>
+    do pG' <- simple_subst_to_pf_env G';
+       pG <- simple_subst_to_pf_env G;
+       ret (pcon "sub" [:: pG'; pG])
+  | scon "el" [:: A; G] =>
+    do pa <- simple_subst_to_pf_ty A;
+       pG <- simple_subst_to_pf_env G;
+       ret (pcon "el" [:: pa; pG])
+  | _ => None
+  end.
+
+Fixpoint simple_subst_to_pf_sub (c : pf_ctx) (e :exp) G_l : option (pf * pf) :=
+  match e with
+  | var x =>
+    do (pcon "sub" [:: G_r;_]) <- named_list_lookup_err c x;
+       ret (pvar x, G_r)
+  | con "id" [::] =>
+    do ret (pcon "id" [:: G_l], G_l)
+  | con "cmp" [:: g; f] =>
+    do (p_f,G_fr) <- simple_subst_to_pf_sub c f G_l;
+       (p_g, G_gr) <- simple_subst_to_pf_sub c g G_fr;
+       ret (pcon "cmp" [:: p_g; p_f; G_gr; G_fr; G_l], G_gr)
+  | con "forget" [::] =>
+    do ret (pcon "forget" [:: G_l], pcon "emp" [::])
+  | con "snoc" [:: e; f] =>
+    do (p_f,G_fr) <- simple_subst_to_pf_sub c f G_l;
+       (p_e, pA) <- simple_subst_to_pf_el c e G_l;
+       ret (pcon "snoc" [:: p_e; p_f; pA; G_fr; G_l], pcon "ext" [:: pA; G_fr])
+  | con "wkn" [::] =>
+    do (pcon "ext" [:: A; G]) <- Some G_l;
+       ret (pcon "wkn" [:: A; G], G)
+  | _ => None
+  end
+with simple_subst_to_pf_el c e G : option (pf * pf) :=
+       match e with
+       | var x =>
+         do (pcon "el" [:: A; _]) <- named_list_lookup_err c x;
+         ret (pvar x, A)
+       | con "el_subst" [:: e; f] =>
+         do (p_f,G_fr) <- simple_subst_to_pf_sub c f G;
+            (p_e, pA) <- simple_subst_to_pf_el c e G_fr;
+            ret (pcon "el_subst" [:: p_e; pA; p_f; G_fr; G], pA)
+      | con "hd" [::] =>
+        do (pcon "ext" [:: A; G]) <- Some G;
+           ret (pcon "hd" [:: A; G], A)
+       | _ => None
+       end.
+
+
+Definition simple_subst_to_pf_term (c : pf_ctx) (e :exp) t : option pf :=
+  match t with
+  | pcon "env" [::] => simple_subst_to_pf_env e
+  | pcon "ty" [::] => simple_subst_to_pf_ty e
+  | pcon "sub" [:: _ ; G_l] =>
+    do (p,_) <- simple_subst_to_pf_sub c e G_l;
+       ret p
+  | pcon "el" [:: _ ; G] =>
+    do (p,_) <- simple_subst_to_pf_el c e G;
+       ret p
+  | _ => None
+  end.
+
+Fixpoint simple_subst_to_pf_ctx (c : ctx) : option pf_ctx :=
+  match c with
+  | [::] => do ret [::]
+  | (n,t)::c' =>
+    do pc' <- simple_subst_to_pf_ctx c';
+       pt <- simple_subst_to_pf_sort t;
+       ret (n,pt)::pc'
+  end.
+
+Definition simple_subst_to_pf_rule (r : rule) : option rule_pf :=
+  match r with
+  | sort_rule c args =>
+    do pc <- simple_subst_to_pf_ctx c;
+    ret sort_rule_pf pc args
+  | term_rule c args t =>
+    do pt <- simple_subst_to_pf_sort t;
+       pc <- simple_subst_to_pf_ctx c;
+    ret term_rule_pf pc args pt
+  | sort_le c t1 t2 =>
+    do pt1 <- simple_subst_to_pf_sort t1;
+       pt2 <- simple_subst_to_pf_sort t2;
+       pc <- simple_subst_to_pf_ctx c;
+    ret sort_le_pf pc pt1 pt2
+  | term_le c e1 e2 t =>
+    do pt <- simple_subst_to_pf_sort t;
+       pc <- simple_subst_to_pf_ctx c;
+       pe1 <- simple_subst_to_pf_term pc e1 pt;
+       pe2 <- simple_subst_to_pf_term pc e2 pt;
+    ret term_le_pf pc pe1 pe2 pt
+end.
+
+Fixpoint simple_subst_to_pf_lang (l : lang) : option pf_lang :=
+  match l with
+  | [::] => do ret [::]
+  | (n,r)::l' =>
+    do pl' <- simple_subst_to_pf_lang l';
+       pr <- simple_subst_to_pf_rule r;
+       ret (n,pr)::pl'
+  end.
+
+
+Ltac prove_wf_with_fn f :=
+  match goal with
+    [|- wf_lang ?l] =>
+    remember (f l) as mp eqn:Heqmp;
+    vm_compute in Heqmp;
+    match goal with
+      [ H : _ = Some ?pl|-_] =>
+      pose (p:=pl); clear H;
+      apply (@synth_wf_lang_related p)
+    end
+  end;
+  by compute.
+
+Lemma simplesubst_wf : wf_lang subst_lang.
+Proof.
+  prove_wf_with_fn simple_subst_to_pf_lang.
+Qed.
